More work on small-step semantics

src/Eval.v
@@ -1,6 +1,7 @@
 Require Import
   Coq.Unicode.Utf8
   Coq.Lists.List
+  Coq.Logic.Classical
   Ty
   Exp
   Sub
@@ -26,7 +27,7 @@ Inductive Step : ∀ {τ}, Exp [] τ → Exp [] τ → Prop :=
     Seq e1 e2 ---> e2
 
   | ST_ListElem τ (l : list (Exp [] τ)) l' pre post x x' :
-    l  = pre ++ x :: post →
+    l  = pre ++ x  :: post →
     l' = pre ++ x' :: post →
     x ---> x' →
     List l ---> List l'
@@ -35,7 +36,7 @@ Inductive Step : ∀ {τ}, Exp [] τ → Exp [] τ → Prop :=
     Let x body ---> APP (LAM body) x
 
   | ST_AppAbs dom cod (e : Exp [dom] cod) (v : Exp [] dom) :
-    ValueP [] dom v ->
+    ValueP v ->
     APP (LAM e) v ---> STmExp {| v |} e
 
   | ST_App1 dom cod (e1 : Exp [] (dom ⟶ cod)) e1' (e2 : Exp [] dom) :
@@ -65,5 +66,87 @@ Proof.
   - now rewrite IHStep.
   - now rewrite IHStep.
 Qed.
+
+Definition normal_form {X : Type}
+           (R : relation X) (t : X) : Prop :=
+  ¬ ∃ t', R t t'.
+
+Lemma app_cons A (y : A) (xs ys : list A) :
+  xs ++ y :: ys = (xs ++ [y]) ++ ys.
+Proof.
+  induction xs; simpl; auto.
+  now rewrite IHxs.
+Qed.
+
+Lemma value_is_nf {τ} (v : Exp [] τ) :
+  ValueP v → normal_form Step v.
+Proof.
+  intros.
+  induction H; intro.
+  - destruct H.
+    now inversion H.
+  - destruct H0.
+    generalize dependent x.
+    induction H; intros.
+    + inversion H0.
+      apply inj_pair2 in H1, H2; subst.
+      apply app_eq_nil in H1.
+      destruct H1.
+      now inversion H1.
+    + inversion H1.
+      apply inj_pair2 in H3, H4; subst.
+      destruct pre.
+      * simpl in *.
+        inversion H3; subst.
+        admit.
+      * admit.
+  - destruct H.
+    now inversion H.
+Abort.
+
+Theorem strong_progress {τ} (e : Exp [] τ) :
+  ValueP e ∨ ∃ e', e ---> e'.
+Proof.
+  dependent elimination e.
+  - now left; constructor.
+  - right.
+    eexists e0.
+    now constructor.
+  - induction l0; simpl.
+    + now left; constructor.
+    + destruct IHl0.
+      * destruct (classic (ValueP a)).
+        ** left.
+           constructor.
+           *** constructor; auto.
+               inversion H; subst.
+               apply inj_pair2 in H2.
+               now subst.
+        ** right.
+           admit.
+      * destruct H.
+        inversion H; subst.
+        apply inj_pair2 in H1; subst.
+        apply inj_pair2 in H2; subst.
+        right.
+        exists (List (a :: pre ++ x' :: post)).
+        rewrite !app_comm_cons.
+        now eapply ST_ListElem; eauto.
+Abort.
+
+Definition deterministic {X : Type} (R : relation X) :=
+  ∀ x y1 y2 : X, R x y1 → R x y2 → y1 = y2.
+
+Theorem step_deterministic τ :
+  deterministic (@Step τ).
+Abort.
+
+Lemma nf_is_value τ (v : Exp [] τ) :
+  normal_form Step v → ValueP v.
+Abort.
+
+Corollary nf_same_as_value τ (v : Exp [] τ) :
+  normal_form Step v ↔ ValueP v.
+Abort.
 
 End Eval.
